matmul_gpu -> mmcomb_gpu

src/lib/inst/gemm/Kuiper.GEMM.Naive2.fst
@@ -9,22 +9,22 @@ open Kuiper.Poly.GEMMCPU {
 open Kuiper.Matrix.Reprs { row_major as RM, col_major as CM }
 module P = Kuiper.Poly.GEMM.Naive2
 
-let matmul_f32_rrr = spec_cpu P.matmul_gpu f32 RM RM RM
-let matmul_f64_rrr = spec_cpu P.matmul_gpu f64 RM RM RM
-let matmul_u32_rrr = spec_cpu P.matmul_gpu u32 RM RM RM
-let matmul_u64_rrr = spec_cpu P.matmul_gpu u64 RM RM RM
+let matmul_f32_rrr = spec_cpu P.mmcomb_gpu f32 RM RM RM
+let matmul_f64_rrr = spec_cpu P.mmcomb_gpu f64 RM RM RM
+let matmul_u32_rrr = spec_cpu P.mmcomb_gpu u32 RM RM RM
+let matmul_u64_rrr = spec_cpu P.mmcomb_gpu u64 RM RM RM
 
-let matmul_f32_ccc = spec_cpu P.matmul_gpu f32 CM CM CM
-let matmul_f64_ccc = spec_cpu P.matmul_gpu f64 CM CM CM
-let matmul_u32_ccc = spec_cpu P.matmul_gpu u32 CM CM CM
-let matmul_u64_ccc = spec_cpu P.matmul_gpu u64 CM CM CM
+let matmul_f32_ccc = spec_cpu P.mmcomb_gpu f32 CM CM CM
+let matmul_f64_ccc = spec_cpu P.mmcomb_gpu f64 CM CM CM
+let matmul_u32_ccc = spec_cpu P.mmcomb_gpu u32 CM CM CM
+let matmul_u64_ccc = spec_cpu P.mmcomb_gpu u64 CM CM CM
 
-let g_matmul_f32_rrr = spec_gpu P.matmul_gpu f32 RM RM RM
-let g_matmul_f64_rrr = spec_gpu P.matmul_gpu f64 RM RM RM
-let g_matmul_u32_rrr = spec_gpu P.matmul_gpu u32 RM RM RM
-let g_matmul_u64_rrr = spec_gpu P.matmul_gpu u64 RM RM RM
+let g_matmul_f32_rrr = spec_gpu P.mmcomb_gpu f32 RM RM RM
+let g_matmul_f64_rrr = spec_gpu P.mmcomb_gpu f64 RM RM RM
+let g_matmul_u32_rrr = spec_gpu P.mmcomb_gpu u32 RM RM RM
+let g_matmul_u64_rrr = spec_gpu P.mmcomb_gpu u64 RM RM RM
 
-let g_matmul_f32_ccc = spec_gpu P.matmul_gpu f32 CM CM CM
-let g_matmul_f64_ccc = spec_gpu P.matmul_gpu f64 CM CM CM
-let g_matmul_u32_ccc = spec_gpu P.matmul_gpu u32 CM CM CM
-let g_matmul_u64_ccc = spec_gpu P.matmul_gpu u64 CM CM CM
+let g_matmul_f32_ccc = spec_gpu P.mmcomb_gpu f32 CM CM CM
+let g_matmul_f64_ccc = spec_gpu P.mmcomb_gpu f64 CM CM CM
+let g_matmul_u32_ccc = spec_gpu P.mmcomb_gpu u32 CM CM CM
+let g_matmul_u64_ccc = spec_gpu P.mmcomb_gpu u64 CM CM CM
