src/lib/inst/gemm/Kuiper.GEMM.BlockTiling1D.fsti
@@ -39,24 +39,24 @@ val matmul_u64_tile16_ccc : fixed_repr_matmul_cpu_ty u64 CM CM CM
 
 (* Specialized to tile=32 *)
 
-val g_matmul_f32_tile32_rrr : fixed_repr_matmul_gpu_ty f32 RM RM RM
-val g_matmul_f64_tile32_rrr : fixed_repr_matmul_gpu_ty f64 RM RM RM
-val g_matmul_u32_tile32_rrr : fixed_repr_matmul_gpu_ty u32 RM RM RM
-val g_matmul_u64_tile32_rrr : fixed_repr_matmul_gpu_ty u64 RM RM RM
+val g_matmul_f32_tile32_rrr : fixed_repr_mmcomb_gpu_ty f32 RM RM RM
+val g_matmul_f64_tile32_rrr : fixed_repr_mmcomb_gpu_ty f64 RM RM RM
+val g_matmul_u32_tile32_rrr : fixed_repr_mmcomb_gpu_ty u32 RM RM RM
+val g_matmul_u64_tile32_rrr : fixed_repr_mmcomb_gpu_ty u64 RM RM RM
 
-val g_matmul_f32_tile32_ccc : fixed_repr_matmul_gpu_ty f32 CM CM CM
-val g_matmul_f64_tile32_ccc : fixed_repr_matmul_gpu_ty f64 CM CM CM
-val g_matmul_u32_tile32_ccc : fixed_repr_matmul_gpu_ty u32 CM CM CM
-val g_matmul_u64_tile32_ccc : fixed_repr_matmul_gpu_ty u64 CM CM CM
+val g_matmul_f32_tile32_ccc : fixed_repr_mmcomb_gpu_ty f32 CM CM CM
+val g_matmul_f64_tile32_ccc : fixed_repr_mmcomb_gpu_ty f64 CM CM CM
+val g_matmul_u32_tile32_ccc : fixed_repr_mmcomb_gpu_ty u32 CM CM CM
+val g_matmul_u64_tile32_ccc : fixed_repr_mmcomb_gpu_ty u64 CM CM CM
 
 (* Specialized to tile=16 *)
 
-val g_matmul_f32_tile16_rrr : fixed_repr_matmul_gpu_ty f32 RM RM RM
-val g_matmul_f64_tile16_rrr : fixed_repr_matmul_gpu_ty f64 RM RM RM
-val g_matmul_u32_tile16_rrr : fixed_repr_matmul_gpu_ty u32 RM RM RM
-val g_matmul_u64_tile16_rrr : fixed_repr_matmul_gpu_ty u64 RM RM RM
+val g_matmul_f32_tile16_rrr : fixed_repr_mmcomb_gpu_ty f32 RM RM RM
+val g_matmul_f64_tile16_rrr : fixed_repr_mmcomb_gpu_ty f64 RM RM RM
+val g_matmul_u32_tile16_rrr : fixed_repr_mmcomb_gpu_ty u32 RM RM RM
+val g_matmul_u64_tile16_rrr : fixed_repr_mmcomb_gpu_ty u64 RM RM RM
 
-val g_matmul_f32_tile16_ccc : fixed_repr_matmul_gpu_ty f32 CM CM CM
-val g_matmul_f64_tile16_ccc : fixed_repr_matmul_gpu_ty f64 CM CM CM
-val g_matmul_u32_tile16_ccc : fixed_repr_matmul_gpu_ty u32 CM CM CM
-val g_matmul_u64_tile16_ccc : fixed_repr_matmul_gpu_ty u64 CM CM CM
+val g_matmul_f32_tile16_ccc : fixed_repr_mmcomb_gpu_ty f32 CM CM CM
+val g_matmul_f64_tile16_ccc : fixed_repr_mmcomb_gpu_ty f64 CM CM CM
+val g_matmul_u32_tile16_ccc : fixed_repr_mmcomb_gpu_ty u32 CM CM CM
+val g_matmul_u64_tile16_ccc : fixed_repr_mmcomb_gpu_ty u64 CM CM CM
