src/lib/inst/gemm/Kuiper.GEMM.Tiled.fsti
@@ -45,36 +45,36 @@ val matmul_u64_tile16_ccc : fixed_repr_matmul_cpu_ty u64 CM CM CM
 
 (* Below are GPU-side versions: they take live GPU pointers and do not memcpy. *)
 
-val g_matmul_f32_rrr (tile : valid_tile) : fixed_repr_matmul_gpu_ty f32 RM RM RM
-val g_matmul_f64_rrr (tile : valid_tile) : fixed_repr_matmul_gpu_ty f64 RM RM RM
-val g_matmul_u32_rrr (tile : valid_tile) : fixed_repr_matmul_gpu_ty u32 RM RM RM
-val g_matmul_u64_rrr (tile : valid_tile) : fixed_repr_matmul_gpu_ty u64 RM RM RM
+val g_matmul_f32_rrr (tile : valid_tile) : fixed_repr_mmcomb_gpu_ty f32 RM RM RM
+val g_matmul_f64_rrr (tile : valid_tile) : fixed_repr_mmcomb_gpu_ty f64 RM RM RM
+val g_matmul_u32_rrr (tile : valid_tile) : fixed_repr_mmcomb_gpu_ty u32 RM RM RM
+val g_matmul_u64_rrr (tile : valid_tile) : fixed_repr_mmcomb_gpu_ty u64 RM RM RM
 
-val g_matmul_f32_ccc (tile : valid_tile) : fixed_repr_matmul_gpu_ty f32 CM CM CM
-val g_matmul_f64_ccc (tile : valid_tile) : fixed_repr_matmul_gpu_ty f64 CM CM CM
-val g_matmul_u32_ccc (tile : valid_tile) : fixed_repr_matmul_gpu_ty u32 CM CM CM
-val g_matmul_u64_ccc (tile : valid_tile) : fixed_repr_matmul_gpu_ty u64 CM CM CM
+val g_matmul_f32_ccc (tile : valid_tile) : fixed_repr_mmcomb_gpu_ty f32 CM CM CM
+val g_matmul_f64_ccc (tile : valid_tile) : fixed_repr_mmcomb_gpu_ty f64 CM CM CM
+val g_matmul_u32_ccc (tile : valid_tile) : fixed_repr_mmcomb_gpu_ty u32 CM CM CM
+val g_matmul_u64_ccc (tile : valid_tile) : fixed_repr_mmcomb_gpu_ty u64 CM CM CM
 
 (* Specialized to tile=32 *)
 
-val g_matmul_f32_tile32_rrr : fixed_repr_matmul_gpu_ty f32 RM RM RM
-val g_matmul_f64_tile32_rrr : fixed_repr_matmul_gpu_ty f64 RM RM RM
-val g_matmul_u32_tile32_rrr : fixed_repr_matmul_gpu_ty u32 RM RM RM
-val g_matmul_u64_tile32_rrr : fixed_repr_matmul_gpu_ty u64 RM RM RM
+val g_matmul_f32_tile32_rrr : fixed_repr_mmcomb_gpu_ty f32 RM RM RM
+val g_matmul_f64_tile32_rrr : fixed_repr_mmcomb_gpu_ty f64 RM RM RM
+val g_matmul_u32_tile32_rrr : fixed_repr_mmcomb_gpu_ty u32 RM RM RM
+val g_matmul_u64_tile32_rrr : fixed_repr_mmcomb_gpu_ty u64 RM RM RM
 
-val g_matmul_f32_tile32_ccc : fixed_repr_matmul_gpu_ty f32 CM CM CM
-val g_matmul_f64_tile32_ccc : fixed_repr_matmul_gpu_ty f64 CM CM CM
-val g_matmul_u32_tile32_ccc : fixed_repr_matmul_gpu_ty u32 CM CM CM
-val g_matmul_u64_tile32_ccc : fixed_repr_matmul_gpu_ty u64 CM CM CM
+val g_matmul_f32_tile32_ccc : fixed_repr_mmcomb_gpu_ty f32 CM CM CM
+val g_matmul_f64_tile32_ccc : fixed_repr_mmcomb_gpu_ty f64 CM CM CM
+val g_matmul_u32_tile32_ccc : fixed_repr_mmcomb_gpu_ty u32 CM CM CM
+val g_matmul_u64_tile32_ccc : fixed_repr_mmcomb_gpu_ty u64 CM CM CM
 
 (* Specialized to tile=16 *)
 
-val g_matmul_f32_tile16_rrr : fixed_repr_matmul_gpu_ty f32 RM RM RM
-val g_matmul_f64_tile16_rrr : fixed_repr_matmul_gpu_ty f64 RM RM RM
-val g_matmul_u32_tile16_rrr : fixed_repr_matmul_gpu_ty u32 RM RM RM
-val g_matmul_u64_tile16_rrr : fixed_repr_matmul_gpu_ty u64 RM RM RM
+val g_matmul_f32_tile16_rrr : fixed_repr_mmcomb_gpu_ty f32 RM RM RM
+val g_matmul_f64_tile16_rrr : fixed_repr_mmcomb_gpu_ty f64 RM RM RM
+val g_matmul_u32_tile16_rrr : fixed_repr_mmcomb_gpu_ty u32 RM RM RM
+val g_matmul_u64_tile16_rrr : fixed_repr_mmcomb_gpu_ty u64 RM RM RM
 
-val g_matmul_f32_tile16_ccc : fixed_repr_matmul_gpu_ty f32 CM CM CM
-val g_matmul_f64_tile16_ccc : fixed_repr_matmul_gpu_ty f64 CM CM CM
-val g_matmul_u32_tile16_ccc : fixed_repr_matmul_gpu_ty u32 CM CM CM
-val g_matmul_u64_tile16_ccc : fixed_repr_matmul_gpu_ty u64 CM CM CM
+val g_matmul_f32_tile16_ccc : fixed_repr_mmcomb_gpu_ty f32 CM CM CM
+val g_matmul_f64_tile16_ccc : fixed_repr_mmcomb_gpu_ty f64 CM CM CM
+val g_matmul_u32_tile16_ccc : fixed_repr_mmcomb_gpu_ty u32 CM CM CM
+val g_matmul_u64_tile16_ccc : fixed_repr_mmcomb_gpu_ty u64 CM CM CM
